Correctness, now also for predicate logics

Abstract_Formula.thy
@@ -11,6 +11,7 @@ lift_definition fset_from_list :: "'a list => 'a fset" is set by (rule finite_se
 lemma mem_fset_from_list[simp]: "x |\<in>| fset_from_list l  \<longleftrightarrow> x \<in> set l" by transfer rule
 lemma fimage_fset_from_list[simp]: "f |`| fset_from_list l = fset_from_list (map f l)"  by transfer auto
 lemma fset_fset_from_list[simp]: "fset (fset_from_list l) = set l"  by transfer auto
+lemmas fset_simps[simp] = set_simps[Transfer.transferred]
 end
 
 locale Abstract_Formulas =
@@ -21,8 +22,13 @@ locale Abstract_Formulas =
   fixes ran_fv :: "'subst \<Rightarrow> ('var \<times> 'annot) set"
   fixes closed :: "'preform \<Rightarrow> bool"
   assumes annotate_preserves_fv: "fst ` fv (freshen a pf) = pre_fv pf"
+  assumes subst_no_vars: "pre_fv pf = {} \<Longrightarrow> fv (subst s f) = {}"
   assumes fv_subst: "fv (subst s f) \<subseteq> ran_fv s"
+  assumes closed_pre_fv: "closed pf \<Longrightarrow> pre_fv pf = {}"
   assumes closed_eq: "closed pf \<Longrightarrow> subst s1 (freshen a1 pf) = subst s2 (freshen a2 pf)"
+begin
+  definition freshenV :: "'annot \<Rightarrow> 'var \<Rightarrow>  ('var \<times> 'annot)" where "freshenV a v = (v,a)"
+end
 
 datatype ('preform, 'var) antecedent =
   Antecedent (a_hyps: "'preform fset") (a_conc: "'preform") (a_fresh: "'var set")
